proof/correctness/1024/avx2/MLKEM_PolyVec_avx2_proof.ec
@@ -67,12 +67,14 @@ proof.
 
   move => [#] ???sgnd_bnd_bp_2 result_2 [#] sgnd_bnd_res_2 res_2_def.
   split.
-  + rewrite !tP;do split; move => *; rewrite !initiE /= // ?mapiE //=;
+  + rewrite !tP;do split; move =>  i ib; rewrite !initiE /= // ?mapiE //=;
+        have := res_2_def i ib;
      by  smt(Array256.initiE Array1024.initiE Array1024.set_eqiE Array1024.set_neqiE).
 
   move => [#] ???sgnd_bnd_bp_3 result_3 [#] sgnd_bnd_res_3 res_3_def.
   split.
-  + rewrite !tP;do split; move => *; rewrite !initiE /= // ?mapiE //=;
+  + rewrite !tP;do split; move =>  i ib; rewrite !initiE /= // ?mapiE //=;
+        have := res_3_def i ib;
      by  smt(Array256.initiE Array1024.initiE Array1024.set_eqiE Array1024.set_neqiE).
 
   move => [#] ??? sgnd_bnd_bp_4 result_4 [#] sgnd_bnd_res_4 res_4_def.
